normalize s->v; add hints

chapter03/demos/demo01.dfy
@@ -5,26 +5,26 @@
 
 datatype SwitchState = On | Off
 
-datatype State = State(switch:SwitchState)
+datatype Variables = Variables(switch:SwitchState)
 
-predicate Init(s:State) {
-    s.switch == Off
+predicate Init(v:Variables) {
+    v.switch == Off
 }
 
-predicate Activate(s:State, s':State) {
-    s'.switch == On
+predicate Activate(v:Variables, v':Variables) {
+    v'.switch == On
 }
 
-predicate Deactivate(s:State, s':State) {
-    s'.switch == Off
+predicate Deactivate(v:Variables, v':Variables) {
+    v'.switch == Off
 }
 
-predicate Toggle(s:State, s':State) {
-    s'.switch == if s.switch.On? then Off else On
+predicate Toggle(v:Variables, v':Variables) {
+    v'.switch == if v.switch.On? then Off else On
 }
 
-predicate Next(s:State, s':State) {
-    || Activate(s, s')
-    || Deactivate(s, s')
-    || Toggle(s, s')
+predicate Next(v:Variables, v':Variables) {
+    || Activate(v, v')
+    || Deactivate(v, v')
+    || Toggle(v, v')
 }
