chapter03/exercises/exercise02.dfy
@@ -19,7 +19,7 @@
 datatype Constants = Constants(tableSize:nat)
 
 //#elide datatype Pair = Pair(left:bool, right:bool)
-datatype State = State(
+datatype Variables = Variables(
 //#elide     philosophers:seq<Pair>
 )
 
@@ -27,45 +27,45 @@ predicate WellFormedConstants(c:Constants) {
     && 0 < c.tableSize 
 }
 
-predicate WellFormed(c:Constants, s:State) {
+predicate WellFormed(c:Constants, v:Variables) {
     && WellFormedConstants(c)
-//#elide    && |s.philosophers| == c.tableSize
+//#elide    && |v.philosophers| == c.tableSize
 }
 
-predicate Init(c:Constants, s:State) {
-//#elide    && WellFormed(c, s)
-//#elide    && (forall pi | 0 <= pi < |s.philosophers| :: s.philosophers[pi] == Pair(false, false))
+predicate Init(c:Constants, v:Variables) {
+//#elide    && WellFormed(c, v)
+//#elide    && (forall pi | 0 <= pi < |v.philosophers| :: v.philosophers[pi] == Pair(false, false))
 }
 
-predicate AcquireLeft(c:Constants, s:State, s':State, pi:nat) {
-//#elide    && WellFormed(c, s)
+predicate AcquireLeft(c:Constants, v:Variables, v':Variables, pi:nat) {
+//#elide    && WellFormed(c, v)
 //#elide    && pi < c.tableSize
-//#elide    && !(s.philosophers[pi].left) // prevents this action from being a no-op
-//#elide    && !(s.philosophers[PhilosopherToTheLeftOf(c,pi)].right) // comment this line to create bug
-//#elide    && s' == s.(philosophers := s.philosophers[pi := Pair(true, s.philosophers[pi].right)])
+//#elide    && !(v.philosophers[pi].left) // prevents this action from being a no-op
+//#elide    && !(v.philosophers[PhilosopherToTheLeftOf(c,pi)].right) // comment this line to create bug
+//#elide    && v' == v.(philosophers := v.philosophers[pi := Pair(true, v.philosophers[pi].right)])
 }
 
-predicate AcquireRight(c:Constants, s:State, s':State, pi:nat) {
-//#elide    && WellFormed(c, s)
+predicate AcquireRight(c:Constants, v:Variables, v':Variables, pi:nat) {
+//#elide    && WellFormed(c, v)
 //#elide    && pi < c.tableSize
-//#elide    && !(s.philosophers[pi].right) // prevents this action from being a no-op
-//#elide    && !(s.philosophers[PhilosopherToTheRightOf(c,pi)].left) // comment this line to create bug
-//#elide    && s' == s.(philosophers := s.philosophers[pi := Pair(s.philosophers[pi].left, true)])
+//#elide    && !(v.philosophers[pi].right) // prevents this action from being a no-op
+//#elide    && !(v.philosophers[PhilosopherToTheRightOf(c,pi)].left) // comment this line to create bug
+//#elide    && v' == v.(philosophers := v.philosophers[pi := Pair(v.philosophers[pi].left, true)])
 }
 
-predicate ReleaseBoth(c:Constants, s:State, s':State, pi:nat) {
-//#elide    && WellFormed(c, s)
+predicate ReleaseBoth(c:Constants, v:Variables, v':Variables, pi:nat) {
+//#elide    && WellFormed(c, v)
 //#elide    && pi < c.tableSize
-//#elide    && (s.philosophers[pi].left)
-//#elide    && (s.philosophers[pi].right)
-//#elide    && s' == s.(philosophers := s.philosophers[pi := Pair(false, false)])
+//#elide    && (v.philosophers[pi].left)
+//#elide    && (v.philosophers[pi].right)
+//#elide    && v' == v.(philosophers := v.philosophers[pi := Pair(false, false)])
 }
  
-predicate Next(c:Constants, s:State, s':State) {
+predicate Next(c:Constants, v:Variables, v':Variables) {
 //#elide    exists pi:nat :: 
-//#elide    (|| AcquireLeft(c, s, s', pi)
-//#elide     || AcquireRight(c, s, s', pi)
-//#elide     || ReleaseBoth(c, s, s', pi))
+//#elide    (|| AcquireLeft(c, v, v', pi)
+//#elide     || AcquireRight(c, v, v', pi)
+//#elide     || ReleaseBoth(c, v, v', pi))
 }
 
 //#elidefunction PhilosopherToTheLeftOf(c:Constants, i:nat) : nat 
@@ -81,35 +81,35 @@ predicate Next(c:Constants, s:State, s':State) {
 //#elide}
 //#elide
 //#elide// here is the safety property
-//#elidepredicate ForkConsistency(c:Constants, s:State) 
+//#elidepredicate ForkConsistency(c:Constants, v:Variables) 
 //#elide{
-//#elide    && WellFormed(c, s)
+//#elide    && WellFormed(c, v)
 //#elide    && (forall i | 0 <= i < c.tableSize :: !(
-//#elide        && s.philosophers[i].right 
-//#elide        && s.philosophers[PhilosopherToTheRightOf(c,i)].left
+//#elide        && v.philosophers[i].right 
+//#elide        && v.philosophers[PhilosopherToTheRightOf(c,i)].left
 //#elide        ))
 //#elide}
 //#elide
 //#elide// here is a proof of the safety property. This lemma should verify
 //#elide// without adding a body 
 //#elidelemma ForkConsistencyLemma() 
-//#elide    ensures forall c, s | Init(c,s) :: ForkConsistency(c, s)
-//#elide    ensures forall c, s, s' | ForkConsistency(c, s) && Next(c, s, s') :: ForkConsistency(c, s')
+//#elide    ensures forall c, v | Init(c,v) :: ForkConsistency(c, v)
+//#elide    ensures forall c, v, v' | ForkConsistency(c, v) && Next(c, v, v') :: ForkConsistency(c, v')
 //#elide{
 //#elide}
 //#elide
 //#elide// this predicate and the following lemma are a way to prevent trivial
 //#elide// specifications of the problem that would prevent a philosopher from
 //#elide// having both forks
-//#elidepredicate PhilosopherHasBothForks(c:Constants, s:State, pi:nat)
+//#elidepredicate PhilosopherHasBothForks(c:Constants, v:Variables, pi:nat)
 //#elide    requires pi < c.tableSize
-//#elide    requires WellFormed(c, s)
+//#elide    requires WellFormed(c, v)
 //#elide{
-//#elide    && s.philosophers[pi].left
-//#elide    && s.philosophers[pi].right
+//#elide    && v.philosophers[pi].left
+//#elide    && v.philosophers[pi].right
 //#elide}
 //#elide
-//#elidelemma PseudoLiveness(c:Constants, pi:nat) returns (b:seq<State>)
+//#elidelemma PseudoLiveness(c:Constants, pi:nat) returns (b:seq<Variables>)
 //#elide    requires c.tableSize == 3
 //#elide    requires pi == 1
 //#elide    ensures 0 < |b| 
@@ -118,9 +118,9 @@ predicate Next(c:Constants, s:State, s':State) {
 //#elide    ensures WellFormed(c, b[|b|-1])
 //#elide    ensures PhilosopherHasBothForks(c, b[|b|-1], pi)
 //#elide{
-//#elide    var s0 := State([Pair(false,false), Pair(false, false), Pair(false, false)]);
-//#elide    var s1 := State([Pair(false,false), Pair(true, false), Pair(false, false)]);
-//#elide    var s2 := State([Pair(false,false), Pair(true, true), Pair(false, false)]);
+//#elide    var s0 := Variables([Pair(false,false), Pair(false, false), Pair(false, false)]);
+//#elide    var s1 := Variables([Pair(false,false), Pair(true, false), Pair(false, false)]);
+//#elide    var s2 := Variables([Pair(false,false), Pair(true, true), Pair(false, false)]);
 //#elide    assert AcquireLeft(c, s0, s1, 1); // witness
 //#elide    assert AcquireRight(c, s1, s2, 1); // witness
 //#elide    b := [s0, s1, s2];
